[Civl] Some cleanup of Paxos proof (#1046)
Improvements to the modeling of Paxos:
1. Adds the possibility of rejection of Join and Vote requests, which
doubles a modeling of timeouts
2. Makes the loops in ProposeHelper and Conclude terminating even in the
presence of Join and Vote rejections

Improvements to the proof of Paxos:
1. Converted permJoinChannel and permVoteChannel into linear sets; the
responses kept in the map values were redundant.
2. Unified receivedPermissions in ProposeHelper and Conclude into a
single global variable ```usedPermissions``` in preparation to later
simplification of the inductive sequentialization proof.

Source/Concurrency/CivlCoreTypes.cs
@@ -86,8 +86,6 @@ namespace Microsoft.Boogie
 
     public int PendingAsyncStartIndex => ActionDecl.OutParams.Count;
 
-    public Expr ExitCondition => ActionDecl.FindExprAttribute("exit_condition");
-
     public bool TriviallyCommutesWith(Action other)
     {
       return !this.ModifiedGlobalVars.Intersect(other.UsedGlobalVarsInAction).Any() &&
