Test/civl/paxos/PaxosImpl.bpl
@@ -1,12 +1,15 @@
-function Inv (joinedNodes: [Round]NodeSet, voteInfo: [Round]Option VoteInfo, acceptorState: [Node]AcceptorState,
-              permJoinChannel: JoinResponseChannel, permVoteChannel: VoteResponseChannel) : bool
+function {:inline} Inv (joinedNodes: [Round]NodeSet, voteInfo: [Round]Option VoteInfo, acceptorState: [Node]AcceptorState,
+              joinChannel: [Round][JoinResponse]int, joinChannelPermissions: Set Permission,
+              voteChannel: [Round][VoteResponse]int, voteChannelPermissions: Set Permission) : bool
 {
-  (forall p: Permission :: permJoinChannel->dom->val[p] ==> p is JoinPerm &&
-    (var r, n, joinResponse := p->r, p->n, permJoinChannel->val[p];
-      Round(r) && Node(n) &&
+  (forall r: Round, jr: JoinResponse :: 0 <= joinChannel[r][jr] && joinChannel[r][jr] <= 1)
+  &&
+  (forall r: Round, jr1: JoinResponse, jr2: JoinResponse :: jr1->from == jr2->from && joinChannel[r][jr1] > 0 && joinChannel[r][jr2] > 0 ==> jr1 == jr2)
+  &&
+  (forall r: Round, jr: JoinResponse :: joinChannel[r][jr] > 0 ==> Round(r) && Node(jr->from) && Set_Contains(joinChannelPermissions, JoinPerm(r, jr->from)) &&
+    (jr is JoinAccept ==>
       (
-        var from, maxRound, maxValue := joinResponse->from, joinResponse->lastVoteRound, joinResponse->lastVoteValue;
-        n == from &&
+        var from, maxRound, maxValue := jr->from, jr->lastVoteRound, jr->lastVoteValue;
         joinedNodes[r][from] &&
         0 <= maxRound && maxRound < r &&
         (maxRound == 0 || (voteInfo[maxRound] is Some && voteInfo[maxRound]->t->ns[from] && voteInfo[maxRound]->t->value == maxValue)) &&
@@ -15,18 +18,16 @@ function Inv (joinedNodes: [Round]NodeSet, voteInfo: [Round]Option VoteInfo, acc
       )
     )
   )
+
   &&
-  (forall p: Permission :: permVoteChannel->dom->val[p] ==> p is VotePerm &&
-    (var r, n, voteResponse := p->r, p->n, permVoteChannel->val[p];
-      Round(r) && Node(n) &&
-      (
-        var from := voteResponse->from;
-        n == from &&
-        voteInfo[r] is Some &&
-        voteInfo[r]->t->ns[from]
-      )
-    )
+  (forall r: Round, vr: VoteResponse :: voteChannel[r][vr] > 0 ==> Round(r) && Node(vr->from) && Set_Contains(voteChannelPermissions, VotePerm(r, vr->from)) &&
+    (vr is VoteAccept ==> voteInfo[r] is Some && voteInfo[r]->t->ns[vr->from])
   )
+  &&
+  (forall r: Round, vr: VoteResponse :: 0 <= voteChannel[r][vr] && voteChannel[r][vr] <= 1)
+  &&
+  (forall r: Round, vr1: VoteResponse, vr2: VoteResponse :: vr1->from == vr2->from && voteChannel[r][vr1] > 0 && voteChannel[r][vr2] > 0 ==> vr1 == vr2)
+
   &&
   (forall n: Node :: Node(n) ==>
     (
@@ -40,30 +41,12 @@ function Inv (joinedNodes: [Round]NodeSet, voteInfo: [Round]Option VoteInfo, acc
   )
 }
 
-function InvChannels (joinChannel: [Round][JoinResponse]int, permJoinChannel: JoinResponseChannel,
-                      voteChannel: [Round][VoteResponse]int, permVoteChannel: VoteResponseChannel) : bool
-{
-  (forall r: Round, jr: JoinResponse :: 0 <= joinChannel[r][jr] && joinChannel[r][jr] <= 1) &&
-  (forall r: Round, vr: VoteResponse :: 0 <= voteChannel[r][vr] && voteChannel[r][vr] <= 1) &&
-  (forall r: Round, jr: JoinResponse ::
-    joinChannel[r][jr] > 0 ==>
-      permJoinChannel->dom->val[JoinPerm(r, jr->from)] &&
-      permJoinChannel->val[JoinPerm(r, jr->from)] == jr) &&
-  (forall r: Round, vr: VoteResponse ::
-    voteChannel[r][vr] > 0 ==>
-      permVoteChannel->dom->val[VotePerm(r, vr->from)] &&
-      permVoteChannel->val[VotePerm(r, vr->from)] == vr)
-}
-
 yield invariant {:layer 1} YieldInit({:linear} ps: Set Permission);
 invariant Init(ps, decision);
-invariant InitLow(acceptorState, joinChannel, voteChannel, permJoinChannel, permVoteChannel);
+invariant InitLow(acceptorState, joinChannel, voteChannel, joinChannelPermissions, voteChannelPermissions);
 
 yield invariant {:layer 1} YieldInv();
-invariant Inv(joinedNodes, voteInfo, acceptorState, permJoinChannel, permVoteChannel);
-
-yield invariant {:layer 1} YieldInvChannels();
-invariant InvChannels(joinChannel, permJoinChannel, voteChannel, permVoteChannel);
+invariant Inv(joinedNodes, voteInfo, acceptorState, joinChannel, joinChannelPermissions, voteChannel, voteChannelPermissions);
 
 ////////////////////////////////////////////////////////////////////////////////
 
@@ -98,7 +81,6 @@ StartRound(r: Round, {:layer 1}{:linear_in} r_lin: Set Permission)
 refines A_StartRound;
 requires {:layer 1} Round(r) && r_lin == AllPermissions(r);
 requires call YieldInv();
-requires call YieldInvChannels();
 {
   var n: int;
   var {:layer 1}{:linear} p: One Permission;
@@ -127,61 +109,58 @@ refines A_Join;
 requires {:layer 1} Round(r) && Node(n) && p->val == JoinPerm(r, n);
 requires call YieldInv();
 {
-  var doJoin: bool;
-  var lastVoteRound: Round;
-  var lastVoteValue: Value;
+  var joinResponse: JoinResponse;
 
-  call doJoin, lastVoteRound, lastVoteValue := JoinUpdate(r, n);
-  if (doJoin) {
-    call SendJoinResponse(r, n, lastVoteRound, lastVoteValue);
-    call {:layer 1} permJoinChannel := SendJoinResponseIntro(JoinResponse(n, lastVoteRound, lastVoteValue), p, permJoinChannel);
+  call joinResponse := JoinUpdate(r, n);
+  call SendJoinResponse(r, joinResponse);
+  if (joinResponse is JoinAccept) {
     call {:layer 1} joinedNodes := Copy(joinedNodes[r := joinedNodes[r][n := true]]);
   }
+  call {:layer 1} One_Put(joinChannelPermissions, p);
 }
 
-yield right procedure {:layer 1} ProposeHelper(r: Round) returns (maxRound: Round, maxValue: Value, {:layer 1} ns: NodeSet)
-modifies permJoinChannel, joinChannel;
+yield right procedure {:layer 1} ProposeHelper(r: Round) returns (maxRound: Round, maxValue: Value, count: int, {:layer 1} ns: NodeSet)
+modifies joinChannelPermissions, joinChannel;
 requires {:layer 1} Round(r);
-requires {:layer 1} Inv(joinedNodes, voteInfo, acceptorState, permJoinChannel, permVoteChannel);
-requires {:layer 1} InvChannels(joinChannel, permJoinChannel, voteChannel, permVoteChannel);
+requires {:layer 1} Inv(joinedNodes, voteInfo, acceptorState, joinChannel, joinChannelPermissions, voteChannel, voteChannelPermissions);
 ensures {:layer 1} maxRound == MaxRound(r, ns, voteInfo);
 ensures {:layer 1} Round(maxRound) ==> maxValue == voteInfo[maxRound]->t->value;
-ensures {:layer 1} IsSubset(ns, joinedNodes[r]) && IsQuorum(ns);
-ensures {:layer 1} Inv(joinedNodes, voteInfo, acceptorState, permJoinChannel, permVoteChannel);
-ensures {:layer 1} InvChannels(joinChannel, permJoinChannel, voteChannel, permVoteChannel);
+ensures {:layer 1} count == Cardinality(ns);
+ensures {:layer 1} (forall x: Node :: ns[x] ==> Node(x));
+ensures {:layer 1} IsSubset(ns, joinedNodes[r]);
+ensures {:layer 1} Inv(joinedNodes, voteInfo, acceptorState, joinChannel, joinChannelPermissions, voteChannel, voteChannelPermissions);
 {
-  var count: int;
+  var n: int;
   var joinResponse: JoinResponse;
-  var {:layer 1}{:linear} receivedPermissions: Set Permission;
   var {:layer 1}{:linear} receivedPermission: One Permission;
 
   call {:layer 1} ns := Copy(NoNodes());
-  call {:layer 1} receivedPermissions := InitializePermissions();
+  n := 0;
   count := 0;
   maxRound := 0;
-  while (true)
+  while (n < numNodes)
+  invariant {:layer 1} 0 <= n && n <= numNodes;
   invariant {:layer 1} count == Cardinality(ns);
-  invariant {:layer 1} (forall x: Node :: ns[x] ==> Node(x));
+  invariant {:layer 1} (forall x: Node :: ns[x] ==> Node(x) && usedPermissions->val[JoinPerm(r, x)]);
   invariant {:layer 1} IsSubset(ns, joinedNodes[r]);
-  invariant {:layer 1} receivedPermissions->val == (lambda {:pool "Permission"} x: Permission :: x is JoinPerm && x->r == r && ns[x->n]);
   invariant {:layer 1} maxRound == MaxRound(r, ns, voteInfo);
   invariant {:layer 1} Round(maxRound) ==> maxValue == voteInfo[maxRound]->t->value;
-  invariant {:layer 1} Inv(joinedNodes, voteInfo, acceptorState, permJoinChannel, permVoteChannel);
-  invariant {:layer 1} InvChannels(joinChannel, permJoinChannel, voteChannel, permVoteChannel);
+  invariant {:layer 1} Inv(joinedNodes, voteInfo, acceptorState, joinChannel, joinChannelPermissions, voteChannel, voteChannelPermissions);
   {
     call joinResponse := ReceiveJoinResponse(r);
-    call {:layer 1} receivedPermission, permJoinChannel := ReceiveJoinResponseIntro(r, joinResponse, permJoinChannel);
-    assume {:add_to_pool "Permission", receivedPermission->val} true;
-    call {:layer 1} MaxRoundLemma(voteInfo, r, ns, SingletonNode(receivedPermission->val->n));
-    call {:layer 1} ns := AddToQuorum(ns, receivedPermission->val->n);
-    call {:layer 1} receivedPermissions := AddPermission(receivedPermissions, receivedPermission);
-    count := count + 1;
-    if (joinResponse->lastVoteRound > maxRound) {
-      maxRound := joinResponse->lastVoteRound;
-      maxValue := joinResponse->lastVoteValue;
-    }
-    if (2 * count > numNodes) {
-      break;
+    call {:layer 1} joinChannelPermissions, usedPermissions := MovePermission(JoinPerm(r, joinResponse->from), joinChannelPermissions, usedPermissions);
+    if (joinResponse is JoinAccept) {
+      //assume {:add_to_pool "Permission", JoinPerm(r, joinResponse->from)} true;
+      call {:layer 1} MaxRoundLemma(voteInfo, r, ns, SingletonNode(joinResponse->from));
+      call {:layer 1} ns := AddToQuorum(ns, joinResponse->from);
+      count := count + 1;
+      if (joinResponse->lastVoteRound > maxRound) {
+        maxRound := joinResponse->lastVoteRound;
+        maxValue := joinResponse->lastVoteValue;
+      }
+      if (2 * count > numNodes) {
+        break;
+      }
     }
   }
 }
@@ -191,32 +170,35 @@ Propose(r: Round, {:layer 1}{:linear_in} ps: Set Permission)
 refines A_Propose;
 requires {:layer 1} Round(r) && ps == ProposePermissions(r);
 requires call YieldInv();
-requires call YieldInvChannels();
 {
   var {:layer 1} maxRound: Round;
   var maxValue: Value;
   var {:layer 1} ns: NodeSet;
-  var n: int;
+  var n, count: int;
   var {:layer 1}{:linear} ps': Set Permission;
   var {:layer 1}{:linear} p: One Permission;
   var {:layer 1}{:linear} cp: One Permission;
   var {:layer 1}{:pending_async} PAs:[A_Vote]int;
 
-  call maxRound, maxValue, ns := ProposeHelper(r);
-  assume {:add_to_pool "NodeSet", ns} {:add_to_pool "MaxValue", maxValue} true;
+  call maxRound, maxValue, count, ns := ProposeHelper(r);
   call {:layer 1} ps', cp := SplitConcludePermission(r, ps);
-  n := 1;
-  while (n <= numNodes)
-  invariant {:layer 1} 1 <= n && n <= numNodes+1;
-  invariant {:layer 1} (forall n': Node :: n <= n' && n' <= numNodes ==> ps'->val[VotePerm(r, n')]);
-  invariant {:layer 1} PAs == ToMultiset((lambda pa: A_Vote :: pa->r == r && 1 <= pa->n && pa->n < n && pa->v == maxValue && pa->p->val == VotePerm(pa->r, pa->n)));
-  {
-    call {:layer 1} ps', p := ExtractVotePermission(ps', r, n);
-    async call Vote(r, n, maxValue, p);
-    n := n + 1;
+  if (2 * count > numNodes) {
+    assume {:add_to_pool "NodeSet", ns} {:add_to_pool "MaxValue", maxValue} true;
+    n := 1;
+    while (n <= numNodes)
+    invariant {:layer 1} 1 <= n && n <= numNodes+1;
+    invariant {:layer 1} (forall n': Node :: n <= n' && n' <= numNodes ==> ps'->val[VotePerm(r, n')]);
+    invariant {:layer 1} PAs == ToMultiset((lambda pa: A_Vote :: pa->r == r && 1 <= pa->n && pa->n < n && pa->v == maxValue && pa->p->val == VotePerm(pa->r, pa->n)));
+    {
+      call {:layer 1} ps', p := ExtractVotePermission(ps', r, n);
+      async call Vote(r, n, maxValue, p);
+      n := n + 1;
+    }
+    async call Conclude(r, maxValue, cp);
+    call {:layer 1} voteInfo := Copy(voteInfo[r := Some(VoteInfo(maxValue, NoNodes()))]);
+  } else {
+    call {:layer 1} Set_Put(usedPermissions, ps');
   }
-  async call Conclude(r, maxValue, cp);
-  call {:layer 1} voteInfo := Copy(voteInfo[r := Some(VoteInfo(maxValue, NoNodes()))]);
 }
 
 yield procedure {:layer 1}
@@ -225,15 +207,15 @@ refines A_Vote;
 requires {:layer 1} Round(r) && Node(n) && p->val == VotePerm(r, n);
 requires call YieldInv();
 {
-  var doVote:bool;
+  var voteResponse: VoteResponse;
 
-  call doVote := VoteUpdate(r, n, v);
-  if (doVote) {
-    call SendVoteResponse(r, n);
-    call {:layer 1} permVoteChannel := SendVoteResponseIntro(VoteResponse(n), p, permVoteChannel);
+  call voteResponse := VoteUpdate(r, n, v);
+  call SendVoteResponse(r, voteResponse);
+  if (voteResponse is VoteAccept) {
     call {:layer 1} joinedNodes := Copy(joinedNodes[r := joinedNodes[r][n := true]]);
     call {:layer 1} voteInfo := Copy(voteInfo[r := Some(VoteInfo(voteInfo[r]->t->value, voteInfo[r]->t->ns[n := true]))]);
   }
+  call {:layer 1} One_Put(voteChannelPermissions, p);
 }
 
 yield procedure {:layer 1}
@@ -241,34 +223,32 @@ Conclude(r: Round, v: Value, {:layer 1}{:linear_in} p: One Permission)
 refines A_Conclude;
 requires {:layer 1} Round(r) && p->val == ConcludePerm(r);
 requires call YieldInv();
-requires call YieldInvChannels();
 {
-  var count: int;
+  var n, count: int;
   var voteResponse: VoteResponse;
   var {:layer 1} q: NodeSet;
-  var {:linear} {:layer 1} receivedPermissions: Set Permission;
   var {:linear} {:layer 1} receivedPermission: One Permission;
 
   call {:layer 1} q := Copy(NoNodes());
-  call {:layer 1} receivedPermissions := InitializePermissions();
+  n := 0;
   count := 0;
-  while (true)
+  while (n < numNodes)
+  invariant {:layer 1} 0 <= n && n <= numNodes;
   invariant {:layer 1} count == Cardinality(q);
-  invariant {:layer 1} (forall x: Node :: q[x] ==> Node(x));
+  invariant {:layer 1} (forall x: Node :: q[x] ==> Node(x) && usedPermissions->val[VotePerm(r, x)]);
   invariant {:layer 1} IsSubset(q, voteInfo[r]->t->ns);
-  invariant {:layer 1} receivedPermissions->val == (lambda x: Permission :: x is VotePerm && x->r == r && q[x->n]);
-  invariant {:layer 1} Inv(joinedNodes, voteInfo, acceptorState, permJoinChannel, permVoteChannel);
-  invariant {:layer 1} InvChannels(joinChannel, permJoinChannel, voteChannel, permVoteChannel);
+  invariant {:layer 1} Inv(joinedNodes, voteInfo, acceptorState, joinChannel, joinChannelPermissions, voteChannel, voteChannelPermissions);
   {
     call voteResponse := ReceiveVoteResponse(r);
-    call {:layer 1} receivedPermission, permVoteChannel := ReceiveVoteResponseIntro(r, voteResponse, permVoteChannel);
-    call {:layer 1} q := AddToQuorum(q, receivedPermission->val->n);
-    call {:layer 1} receivedPermissions := AddPermission(receivedPermissions, receivedPermission);
-    count := count + 1;
-    if (2 * count > numNodes) {
-      call {:layer 1} decision := Copy(decision[r := Some(v)]);
-      assume {:add_to_pool "NodeSet", q} true;
-      break;
+    call {:layer 1} voteChannelPermissions, usedPermissions := MovePermission(VotePerm(r, voteResponse->from), voteChannelPermissions, usedPermissions);
+    if (voteResponse is VoteAccept) {
+      call {:layer 1} q := AddToQuorum(q, voteResponse->from);
+      count := count + 1;
+      if (2 * count > numNodes) {
+        call {:layer 1} decision := Copy(decision[r := Some(v)]);
+        assume {:add_to_pool "NodeSet", q} true;
+        break;
+      }
     }
   }
 }
@@ -290,40 +270,44 @@ ensures MaxRound(r, MapOr(ns1, ns2), voteInfo) ==
 
 ////////////////////////////////////////////////////////////////////////////////
 
-yield procedure {:layer 0} JoinUpdate(r: Round, n: Node) returns (join:bool, lastVoteRound: Round, lastVoteValue: Value);
+yield procedure {:layer 0} JoinUpdate(r: Round, n: Node) returns (joinResponse: JoinResponse);
 refines atomic action {:layer 1} _
 {
   var lastJoinRound: Round;
+  var lastVoteRound: Round;
+  var lastVoteValue: Value;
+
   lastJoinRound := acceptorState[n]->lastJoinRound;
   if (r > lastJoinRound) {
     lastVoteRound := acceptorState[n]->lastVoteRound;
     lastVoteValue := acceptorState[n]->lastVoteValue;
     acceptorState[n] := AcceptorState(r, lastVoteRound, lastVoteValue);
-    join := true;
+    joinResponse := JoinAccept(n, lastVoteRound, lastVoteValue);
   } else {
-    join := false;
+    joinResponse := JoinReject(n);
   }
 }
 
-yield procedure {:layer 0} VoteUpdate(r: Round, n: Node, v: Value) returns (vote:bool);
+yield procedure {:layer 0} VoteUpdate(r: Round, n: Node, v: Value) returns (voteResponse: VoteResponse);
 refines atomic action {:layer 1} _
 {
   var lastJoinRound: Round;
+
   lastJoinRound := acceptorState[n]->lastJoinRound;
   if (r >= lastJoinRound) {
     acceptorState[n] := AcceptorState(r, r, v);
-    vote := true;
+    voteResponse := VoteAccept(n);
   } else {
-    vote := false;
+    voteResponse := VoteReject(n);
   }
 }
 
 //// Channel send/receive actions
 
-yield procedure {:layer 0} SendJoinResponse(round: Round, from: Node, lastVoteRound: Round, lastVoteValue: Value);
+yield procedure {:layer 0} SendJoinResponse(round: Round, joinResponse: JoinResponse);
 refines left action {:layer 1} _
 {
-  joinChannel[round][JoinResponse(from, lastVoteRound, lastVoteValue)] := joinChannel[round][JoinResponse(from, lastVoteRound, lastVoteValue)] + 1;
+  joinChannel[round][joinResponse] := joinChannel[round][joinResponse] + 1;
 }
 
 yield procedure {:layer 0} ReceiveJoinResponse(round: Round) returns (joinResponse: JoinResponse);
@@ -333,10 +317,10 @@ refines right action {:layer 1} _
   joinChannel[round][joinResponse] := joinChannel[round][joinResponse] - 1;
 }
 
-yield procedure {:layer 0} SendVoteResponse(round: Round, from: Node);
+yield procedure {:layer 0} SendVoteResponse(round: Round, voteResponse: VoteResponse);
 refines left action {:layer 1} _
 {
-  voteChannel[round][VoteResponse(from)] := voteChannel[round][VoteResponse(from)] + 1;
+  voteChannel[round][voteResponse] := voteChannel[round][voteResponse] + 1;
 }
 
 yield procedure {:layer 0} ReceiveVoteResponse(round: Round) returns (voteResponse: VoteResponse);
@@ -346,41 +330,18 @@ refines right action {:layer 1} _
   voteChannel[round][voteResponse] := voteChannel[round][voteResponse] - 1;
 }
 
-//// Introduction procedures to make send/receive more abstract
-
-pure action SendJoinResponseIntro(joinResponse: JoinResponse, {:linear_in} p: One Permission, {:linear_in} permJoinChannel: JoinResponseChannel)
-returns ({:linear} permJoinChannel': JoinResponseChannel)
-{
-  permJoinChannel' := permJoinChannel;
-  call Map_Put(permJoinChannel', p, joinResponse);
-}
-
-pure action ReceiveJoinResponseIntro(round: Round, joinResponse: JoinResponse, {:linear_in} permJoinChannel: JoinResponseChannel)
-returns ({:linear} receivedPermission: One Permission, {:linear} permJoinChannel': JoinResponseChannel)
-{
-  var _x: JoinResponse;
-
-  permJoinChannel' := permJoinChannel;
-  call receivedPermission, _x := Map_Get(permJoinChannel', JoinPerm(round, joinResponse->from));
-}
-
-pure action SendVoteResponseIntro(voteResponse: VoteResponse, {:linear_in} p: One Permission, {:linear_in} permVoteChannel: VoteResponseChannel)
-returns ({:linear} permVoteChannel': VoteResponseChannel)
-{
-  permVoteChannel' := permVoteChannel;
-  call Map_Put(permVoteChannel', p, voteResponse);
-}
-
-pure action ReceiveVoteResponseIntro(round: Round, voteResponse: VoteResponse, {:linear_in} permVoteChannel: VoteResponseChannel)
-returns ({:linear} receivedPermission: One Permission, {:linear} permVoteChannel': VoteResponseChannel)
-{
-  var _x: VoteResponse;
-
-  permVoteChannel' := permVoteChannel;
-  call receivedPermission, _x := Map_Get(permVoteChannel', VotePerm(round, voteResponse->from));
-}
-
 //// Permission accounting
+
+pure action MovePermission(p: Permission, {:linear_in} from: Set Permission, {:linear_in} to: Set Permission)
+returns ({:linear} from': Set Permission, {:linear} to': Set Permission)
+{
+  var {:linear} one_p: One Permission;
+
+  from' := from;
+  to' := to;
+  call one_p := One_Get(from', p);
+  call One_Put(to', one_p);
+}
 
 pure action ExtractRoundPermission({:linear_in} ps: Set Permission, r: Round)
 returns ({:linear} ps': Set Permission, {:linear} r_lin: Set Permission)
@@ -417,19 +378,6 @@ returns ({:linear} ps': Set Permission, {:linear} p: One Permission)
 {
   ps' := ps;
   call p := One_Get(ps', VotePerm(r, n));
-}
-
-pure action InitializePermissions()
-returns ({:linear} receivedPermissions: Set Permission)
-{
-  call receivedPermissions := Set_MakeEmpty();
-}
-
-pure action AddPermission({:linear_in} receivedPermissions: Set Permission, {:linear_in} p: One Permission)
-returns ({:linear}receivedPermissions': Set Permission)
-{
-  receivedPermissions' := receivedPermissions;
-  call One_Put(receivedPermissions', p);
 }
 
 // Local Variables:
